Experimenting with lift for replaceNats

QuerySMT/ReplaceNats.lean
@@ -14,6 +14,60 @@ syntax (name := replaceNats) "replaceNats" : tactic
 instance : CanLift Nat Int Int.natAbs (fun _ => True) :=
   { prf := (fun x _ => Exists.intro ↑x (Int.natAbs_ofNat x)) }
 
+def intFunToNatFun (g : Int → Int) (n : Nat) : Nat := (g (Int.ofNat n)).natAbs
+def natFunToIntFun (f : Nat → Nat) (z : Int) : Int := Int.ofNat (f z.natAbs)
+def intFunNatFunInv (f : Nat → Nat) : intFunToNatFun (natFunToIntFun f) = f := by
+  unfold intFunToNatFun natFunToIntFun
+  simp only [Int.ofNat_eq_coe, Int.natAbs_ofNat]
+
+instance : CanLift (Nat → Nat) (Int → Int) intFunToNatFun (fun _ => True) :=
+  { prf := (fun f _ => Exists.intro (natFunToIntFun f) (intFunNatFunInv f)) }
+
+def intInputToNatInput (g : Int → α) (n : Nat) : α := g (Int.ofNat n)
+def natInputToIntInput (f : Nat → α) (z : Int) : α := f z.natAbs
+def intInputNatInputInv (f : Nat → α) : intInputToNatInput (natInputToIntInput f) = f := by
+  unfold intInputToNatInput natInputToIntInput
+  simp only [Int.ofNat_eq_coe, Int.natAbs_ofNat]
+
+instance (α) : CanLift (Nat → α) (Int → α) intInputToNatInput (fun _ => True) :=
+  { prf := (fun f _ => Exists.intro (natInputToIntInput f) (intInputNatInputInv f)) }
+
+def intOutputToNatOutput (g : α → Int) (a : α) : Nat := (g a).natAbs
+def natOutputToIntOutput (f : α → Nat) (a : α) : Int := Int.ofNat (f a)
+def intOutputNatOutputInv (f : α → Nat) : intOutputToNatOutput (natOutputToIntOutput f) = f := by
+  unfold intOutputToNatOutput natOutputToIntOutput
+  simp only [Int.ofNat_eq_coe, Int.natAbs_ofNat]
+
+instance (α) : CanLift (α → Nat) (α → Int) intOutputToNatOutput (fun _ => True) :=
+  { prf := (fun f _ => Exists.intro (natOutputToIntOutput f) (intOutputNatOutputInv f)) }
+
+def intProdToNatProd (x : Int × Int) : Nat × Nat := (x.1.natAbs, x.2.natAbs)
+def natProdToIntProd (x : Nat × Nat) : Int × Int := (Int.ofNat x.1, Int.ofNat x.2)
+def intProdNatProdInv (x : Nat × Nat) : intProdToNatProd (natProdToIntProd x) = x := by
+  unfold intProdToNatProd natProdToIntProd
+  simp only [Int.ofNat_eq_coe, Int.natAbs_ofNat]
+
+instance : CanLift (Nat × Nat) (Int × Int) intProdToNatProd (fun _ => True) :=
+  { prf := (fun x _ => Exists.intro (natProdToIntProd x) (intProdNatProdInv x)) }
+
+def intProd1ToNatProd1 (x : Int × α) : Nat × α := (x.1.natAbs, x.2)
+def natProd1ToIntProd1 (x : Nat × α) : Int × α := (Int.ofNat x.1, x.2)
+def intProd1NatProd1Inv (x : Nat × α) : intProd1ToNatProd1 (natProd1ToIntProd1 x) = x := by
+  unfold intProd1ToNatProd1 natProd1ToIntProd1
+  simp only [Int.ofNat_eq_coe, Int.natAbs_ofNat]
+
+instance (α) : CanLift (Nat × α) (Int × α) intProd1ToNatProd1 (fun _ => True) :=
+  { prf := (fun x _ => Exists.intro (natProd1ToIntProd1 x) (intProd1NatProd1Inv x)) }
+
+def intProd2ToNatProd2 (x : α × Int) : α × Nat := (x.1, x.2.natAbs)
+def natProd2ToIntProd2 (x : α × Nat) : α × Int := (x.1, Int.ofNat x.2)
+def intProd2NatProd2Inv (x : α × Nat) : intProd2ToNatProd2 (natProd2ToIntProd2 x) = x := by
+  unfold intProd2ToNatProd2 natProd2ToIntProd2
+  simp only [Int.ofNat_eq_coe, Int.natAbs_ofNat]
+
+instance (α) : CanLift (α × Nat) (α × Int) intProd2ToNatProd2 (fun _ => True) :=
+  { prf := (fun x _ => Exists.intro (natProd2ToIntProd2 x) (intProd2NatProd2Inv x)) }
+
 @[tactic replaceNats]
 def evalReplaceNats : Tactic
 | `(replaceNats | replaceNats) => do
@@ -47,6 +101,7 @@ def evalReplaceNats : Tactic
         evalTactic $ ← `(tactic| clear $eqFactIdent)
         evalTactic $ ← `(tactic| clear $castEqFactIdent)
         evalTactic $ ← `(tactic| clear $nOldIdent)
+    evalTactic $ ← `(tactic| try simp only [Nat.cast, NatCast.natCast] at *)
 | _ => throwUnsupportedSyntax
 
 example (x : Nat) (y : Nat) (z : Int) (h : z = x + y) : z = x + y := by
@@ -56,5 +111,40 @@ example (x : Nat) (y : Nat) (z : Int) (h : z = x + y) : z = x + y := by
 example (f : Nat → Prop) (x : Nat) (h : f 0) (x_eq_zero : x = 0) : f x := by
   replaceNats
   simp only [x_eq_zero, Int.natAbs_zero, h]
+
+example (f : Nat → Prop) (x : Nat × Nat) (h : f 0) (x_eq_zero : x.1 = 0) : f x.1 := by
+  /- Current tests suggest I can only lift `x` to `Int × Int` when I directly define
+     `CanLift (Nat × Nat) (Int × Int)`. It doesn't appear to be sufficient to define
+     `CanLift (Nat × α) (Int × α)` and `CanLift (α × Nat) (α × Int)`. Though it's
+     possible I'm doing something wrong since lift's documentation here
+     (https://leanprover-community.github.io/mathlib4_docs/Mathlib/Tactic/Lift.html#Mathlib.Tactic.lift)
+     appears to suggest that `CanLift` will automatically generate transitive instances -/
+  zify at *
+  lift x to Int × Int using True.intro
+  unfold intProdToNatProd
+  simp only
+  unfold intProdToNatProd at x_eq_zero
+  simp only at x_eq_zero
+  /- I can't get rid of the casting because I don't know that `x.1` is always nonnegative
+     (even though it definitely is since I lifted `x` from `Nat × Nat`) -/
+  sorry
+
+example (f g : Nat → Nat) (h : ∀ x : Nat, f x = g x) : f = g := by
+  /- Current tests suggest I can only lift f to Int → Int when I directly define
+     `CanLift (Nat → Nat) (Int → Int)`. It doesn't appear to be sufficient to define
+     `CanLift (Nat → α) (Int → α)` and `CanLift (α → Nat) (α → Int)`. Though it's
+     possible I'm doing something wrong since lift's documentation here
+     (https://leanprover-community.github.io/mathlib4_docs/Mathlib/Tactic/Lift.html#Mathlib.Tactic.lift)
+     appears to suggest that `CanLift` will automatically generate transitive instances -/
+  zify at *
+  lift f to Int → Int using True.intro
+  lift g to Int → Int using True.intro
+  unfold intFunToNatFun
+  simp only [Int.ofNat_eq_coe]
+  unfold intFunToNatFun at h
+  simp only [Int.ofNat_eq_coe] at h
+  /- I can't get rid of the casting because I don't know that `f` and `g` always output nonnegative
+     results (even though they definitely do since I lifted them from `Nat → Nat`) -/
+  sorry
 
 end ReplaceNats
